Refactor the definition of `Progress`

ReactorModel/Execution/Theorems/Progress.lean
@@ -5,33 +5,43 @@ open Reactor Classical
 
 namespace Execution
 
--- A reactor `rtr` has the progress property, if from any nonterminal state based at `rtr`, we can
--- perform an execution step.
-def Progress [Hierarchical α] (rtr : α) : Prop :=
-  ∀ (s : State.Over rtr), ¬s.Terminal → ∃ s' : State α, s ↓ s'
+variable [Hierarchical α]
+
+-- A state `s` is stuck, if there does not exist a valid execution step starting at `s`.
+def State.Stuck (s : State α) : Prop :=
+  ¬∃ s', Nonempty (Step s s')
+
+theorem State.Stuck.not_iff {s : State α} : ¬s.Stuck ↔ ∃ s', Nonempty (Step s s') := by
+  simp [State.Stuck]
+
+-- A reactor `rtr` has the progress property, if non-terminal states based at `rtr` are not stuck.
+def Progress (rtr : α) : Prop :=
+  ∀ (s : State.Over rtr), ¬s.Terminal → ¬s.Stuck
 
 namespace Progress
-theorem to_deps_acyclic [Hierarchical α] {rtr : α} (p : Progress rtr) : Dependency.Acyclic rtr := by
-  simp [Dependency.Acyclic.iff_mem_acyclic]
+
+theorem to_deps_acyclic {rtr : α} (p : Progress rtr) : Dependency.Acyclic rtr := by
+  simp only [Dependency.Acyclic.iff_mem_acyclic]
   intro rcn hm
-  have ⟨_, ⟨e⟩⟩ := p _ <| State.Over.forcing_not_terminal hm
+  have ⟨_, ⟨e⟩⟩ := State.Stuck.not_iff.mp <| p _ <| State.Over.forcing_not_terminal hm
   cases e
   case time e => exact State.Over.forcing_not_time_step e hm |>.elim
   case skip e => exact State.Over.forcing_skip_step_rcn_eq e ▸ e.allows_rcn.acyclic
   case exec e => exact State.Over.forcing_exec_step_rcn_eq e ▸ e.allows_rcn.acyclic
 
-variable [Proper α] [Reactor.Finite α] {rtr : α}
+variable {α} [Proper α] [Reactor.Finite α] {rtr : α}
 
 theorem of_deps_acyclic (a : Dependency.Acyclic rtr) : Progress rtr :=
   fun s ht =>
-    if hc : s.Closed then
-      let ⟨_, hg⟩ := State.Terminal.not_elim ht |>.resolve_left (not_not.mpr hc)
-      ⟨_, ⟨.time ⟨hc, hg, refresh_correct _ <| Partial.mapIdx_ids ..⟩⟩⟩
-    else
-      let ⟨rcn, hr⟩ := s.exists_allowed_of_acyclic_not_closed a hc
-      if h : s.Triggers rcn
-      then ⟨_, ⟨.exec ⟨hr, h, Step.Apply.RTC.construct .. |>.snd⟩⟩⟩
-      else ⟨_, ⟨.skip ⟨hr, h⟩⟩⟩
+    State.Stuck.not_iff.mpr <|
+      if hc : s.Closed then
+        let ⟨_, hg⟩ := State.Terminal.not_elim ht |>.resolve_left (not_not.mpr hc)
+        ⟨_, ⟨.time ⟨hc, hg, refresh_correct _ <| Partial.mapIdx_ids ..⟩⟩⟩
+      else
+        let ⟨rcn, hr⟩ := s.exists_allowed_of_acyclic_not_closed a hc
+        if h : s.Triggers rcn
+        then ⟨_, ⟨.exec ⟨hr, h, Step.Apply.RTC.construct .. |>.snd⟩⟩⟩
+        else ⟨_, ⟨.skip ⟨hr, h⟩⟩⟩
 
 theorem iff_deps_acyclic : (Progress rtr) ↔ (Dependency.Acyclic rtr) :=
   ⟨to_deps_acyclic, of_deps_acyclic⟩
